fairness/lm_fairness_preservation.v
@@ -4,46 +4,34 @@ From trillium.program_logic Require Export adequacy.
 From trillium.fairness Require Export inftraces fairness fuel traces_match. 
 
 
+(* TODO: move? *)
+Lemma traces_match_LM_preserves_validity `{LM: LiveModel G M}
+  `{C: Type} {L: Type}
+   (otr: trace C L) (auxtr : auxtrace (LM := LM))
+   state_rel lbl_rel outer_step :
+  traces_match lbl_rel state_rel outer_step LM.(lm_ls_trans) otr auxtr ->
+  auxtrace_valid auxtr (LM := LM).
+Proof.
+  revert otr auxtr. cofix CH. intros otr auxtr Hmatch.
+  inversion Hmatch; first by constructor.
+  constructor =>//. by eapply CH.
+Qed.
+
+
 Definition lm_exaux_traces_match `{LM:LiveModel (locale Λ) M} `{EqDecision (locale Λ)} :
-  extrace Λ → auxtrace (M := LM) → Prop :=
+  extrace Λ → auxtrace (LM := LM) → Prop :=
   traces_match labels_match
                live_tids
                locale_step
                LM.(lm_ls_trans).
+
 
 Section fairness_preserved.
   Context `{LM: LiveModel (locale Λ) M}.
   Context `{Countable (locale Λ)}.
   Notation "'Tid'" := (locale Λ).
 
-  Lemma exaux_preserves_validity extr (auxtr : auxtrace (M := LM)):
-    lm_exaux_traces_match extr auxtr ->
-    auxtrace_valid auxtr (LM := LM).
-  Proof.
-    revert extr auxtr. cofix CH. intros extr auxtr Hmatch.
-    inversion Hmatch; first by constructor.
-    constructor =>//. by eapply CH.
-  Qed.
-
-  Lemma exaux_preserves_termination extr (auxtr : auxtrace (M := LM)) :
-    lm_exaux_traces_match extr auxtr ->
-    terminating_trace auxtr ->
-    terminating_trace extr.
-  Proof.
-    intros Hmatch [n HNone].
-    revert extr auxtr Hmatch HNone. induction n as [|n IHn]; first done.
-    intros extr auxtr Hmatch HNone.
-    replace (S n) with (1 + n) in HNone =>//.
-    rewrite (after_sum' _ 1) in HNone.
-    destruct auxtr as [s| s ℓ auxtr'];
-      first by inversion Hmatch; simplify_eq; exists 1.
-    simpl in HNone.
-    inversion Hmatch; simplify_eq.
-    apply terminating_trace_cons.
-    eapply IHn =>//.
-  Qed.
-
-  Lemma traces_match_labels tid ℓ c δ rex (raux : auxtrace (M := LM)) :
+  Lemma traces_match_labels tid ℓ c δ rex (raux : auxtrace (LM := LM)) :
     lm_exaux_traces_match (c -[Some tid]-> rex) (δ -[ℓ]-> raux) ->
     ((∃ ρ, ℓ = Take_step ρ tid) ∨ (ℓ = Silent_step tid)).
   Proof.
@@ -63,7 +51,7 @@ Section fairness_preserved.
   Local Hint Resolve mapping_live_role: core.
   Local Hint Resolve fuel_live_role: core.
 
-  Lemma match_locale_enabled (extr : extrace Λ) (auxtr : auxtrace (M := LM)) ζ ρ:
+  Lemma match_locale_enabled (extr : extrace Λ) (auxtr : auxtrace (LM := LM)) ζ ρ:
     lm_exaux_traces_match extr auxtr ->
     ls_mapping (trfirst auxtr) !! ρ = Some ζ ->
     locale_enabled ζ (trfirst extr).
@@ -79,7 +67,7 @@ Section fairness_preserved.
   Local Hint Resolve match_locale_enabled: core.
   Local Hint Resolve pred_first_trace: core.
 
-  Definition fairness_induction_stmt ρ fm f m ζ extr (auxtr : auxtrace (M := LM))
+  Definition fairness_induction_stmt ρ fm f m ζ extr (auxtr : auxtrace (LM := LM))
     δ c :=
       (infinite_trace extr ->
        (forall ζ, fair_ex ζ extr) ->
@@ -92,10 +80,10 @@ Section fairness_preserved.
       ∃ M, pred_at auxtr M (λ δ _, ¬role_enabled ρ δ)
            ∨ pred_at auxtr M (λ _ ℓ, ∃ ζ0, ℓ = Some (Take_step ρ ζ0))).
 
-  Local Lemma case1 ρ f m (extr' : extrace Λ) (auxtr' : auxtrace (M := LM)) δ ℓ :
+  Local Lemma case1 ρ f m (extr' : extrace Λ) (auxtr' : auxtrace (LM := LM)) δ ℓ :
     (∀ m0 : nat * nat,
          strict lt_lex m0 (f, m)
-         → ∀ (f m: nat) (ζ: locale Λ) (extr : extrace Λ) (auxtr : auxtrace (M := LM))
+         → ∀ (f m: nat) (ζ: locale Λ) (extr : extrace Λ) (auxtr : auxtrace (LM := LM))
              (δ : LiveState Tid M) (c : cfg Λ), fairness_induction_stmt ρ m0 f m ζ extr auxtr δ c) ->
     (ρ ∈ dom (ls_fuel (trfirst auxtr')) → oless (ls_fuel (trfirst auxtr') !! ρ) (ls_fuel δ !! ρ)) ->
     lm_exaux_traces_match extr' auxtr' ->
@@ -126,7 +114,7 @@ Section fairness_preserved.
                                   ∨ pred_at auxtr' M0 (λ (_ : LiveState Tid M) ℓ, ∃ ζ0, ℓ = Some (Take_step ρ ζ0)).
         { eapply (IH _ _ _ p _ extr'); eauto.
           Unshelve. unfold strict, lt_lex. specialize (Hdec ltac:(by eapply elem_of_dom_2)).
-          rewrite Heq in Hdec. lia. }
+          lia. }
         exists (1+P). rewrite !pred_at_sum. simpl. done.
       - exists 1. left. rewrite /pred_at /=. rewrite /role_enabled.
         destruct auxtr' =>/=.
@@ -135,7 +123,7 @@ Section fairness_preserved.
     Qed.
 
   Lemma fairness_preserved_ind ρ:
-    ∀ fm f m ζ (extr: extrace Λ) (auxtr: auxtrace (M := LM)) δ c,
+    ∀ fm f m ζ (extr: extrace Λ) (auxtr: auxtrace (LM := LM)) δ c,
       fairness_induction_stmt ρ fm f m ζ extr auxtr δ c.
   Proof.
     induction fm as [fm IH] using lex_ind.
@@ -264,7 +252,7 @@ Section fairness_preserved.
         exists (1+P). rewrite !pred_at_sum. simpl. done.
   Qed.
 
-  Theorem fairness_preserved (extr: extrace Λ) (auxtr: auxtrace (M := LM)):
+  Theorem fairness_preserved (extr: extrace Λ) (auxtr: auxtrace (LM := LM)):
     infinite_trace extr ->
     lm_exaux_traces_match extr auxtr ->
     (forall ζ, fair_ex ζ extr) -> (forall ρ, fair_aux ρ auxtr (LM := LM)).
@@ -272,9 +260,9 @@ Section fairness_preserved.
     intros Hinfin Hmatch Hex ρ n Hn.
     unfold pred_at in Hn.
     destruct (after n auxtr) as [tr|] eqn:Heq.
-    2: { by rewrite Heq in Hn. } 
+    2: { done. } 
     setoid_rewrite pred_at_sum. rewrite Heq.
-    rewrite Heq in Hn. 
+    (* rewrite Heq in Hn.  *)
     have Hen: role_enabled ρ (trfirst tr) by destruct tr.
     have [ζ Hζ] : is_Some((trfirst tr).(ls_mapping) !! ρ) by eauto.
     have [f Hfuel] : is_Some((trfirst tr).(ls_fuel) !! ρ) by eauto.
